ObcToClight/DataflowElab.v
@@ -14,6 +14,8 @@ Require Import List.
 Import List.ListNotations.
 Open Scope list_scope.
 
+Require compcert.cfrontend.Cop.
+
 Require Import compcert.common.Errors.
 Local Open Scope error_monad_scope.
 
@@ -38,10 +40,9 @@ Definition err_loc (loc: astloc) (m: errmsg) :=
 
 Module Type ELABORATION
        (Import Ids    : IDS)
-       (Import Op     : OPERATORS)
-       (Import OpAux  : OPERATORS_AUX Op)
-       (Import Syn    : SYNTAX Ids Op)
-       (Import Typing : TYPING Ids Op Syn).
+       (Import OpAux  : OPERATORS_AUX Interface.Op)
+       (Import Syn    : SYNTAX Ids Interface.Op)
+       (Import Typing : TYPING Ids Interface.Op Syn).
 
   Definition elab_constant (loc: astloc) (c: Ast.constant) : constant :=
     match c with
@@ -56,53 +57,179 @@ Module Type ELABORATION
 
     Variable env : PM.t type.
 
-    Definition has_type (x: ident) (ty: type) : bool :=
+    Definition find_type (loc: astloc) (x: ident) : res type :=
       match PM.find x env with
-      | Some ty' => ty ==b ty'
-      | None => false
+      | None => Error (err_loc loc (CTX x :: msg " is not declared."))
+      | Some ty => OK ty
       end.
+
+    Definition assert_type (loc: astloc) (x: ident) (ty: type) : res unit :=
+      do xty <- find_type loc x;
+         if xty ==b ty then OK tt
+         else Error (err_loc loc
+                      (CTX x :: MSG " has type " :: MSG (string_of_type xty)
+                             :: MSG " but type " :: MSG (string_of_type ty)
+                             :: MSG " was expected." :: nil)).
 
     Fixpoint elab_clock (loc: astloc) (ck: Ast.clock) : res clock :=
       match ck with
       | BASE => OK Cbase
-      | ON ck' b xs =>
-        let x := ident_of_string xs in
-        if has_type x bool_type then
-          do ck' <- elab_clock loc ck';
-             OK (Con ck' x b)
-        else Error (err_loc loc
-                       (CTX x :: msg " in clock is not declared as bool."))
+      | ON ck' b sx =>
+        let x := ident_of_string sx in
+        do ok <- assert_type loc x bool_type;
+        do ck' <- elab_clock loc ck';
+           OK (Con ck' x b)
+      end.
+
+    Definition elab_unop (op: Ast.unary_operator) : unop :=
+      match op with
+      | MINUS => UnaryOp Cop.Oneg
+      | NOT   => UnaryOp Cop.Onotint
+      | BNOT  => UnaryOp Cop.Onotbool
+      end.
+
+    Definition elab_binop (op: Ast.binary_operator) : binop :=
+      match op with
+      | ADD  => Cop.Oadd
+      | SUB  => Cop.Osub
+      | MUL  => Cop.Omul
+      | DIV  => Cop.Odiv
+      | MOD  => Cop.Omod
+      | BAND => Cop.Oand
+      | BOR  => Cop.Oor
+      | LAND => Cop.Oand
+      | LOR  => Cop.Oor
+      | XOR  => Cop.Oxor
+      | LSL  => Cop.Oshl
+      | LSR  => Cop.Oshr
+      | EQ   => Cop.Oeq
+      | NE   => Cop.One
+      | LT   => Cop.Olt
+      | GT   => Cop.Ogt
+      | LE   => Cop.Ole
+      | GE   => Cop.Oge
+      end.
+
+    (* TODO: fix type_unop' to match completely *)
+    Definition find_type_unop (loc: astloc) (op: unop) (ty: type) : res type :=
+      match type_unop' op ty with
+      | None => Error (err_loc loc (msg "wrong operator argument type"))
+      | Some ty' => OK ty'
+      end.
+
+    Definition find_type_binop (loc: astloc) (op: binop)
+                                             (ty1 ty2: type) : res type :=
+      match type_binop' op ty1 ty2 with
+      | None => Error (err_loc loc (msg "wrong operator argument type"))
+      | Some ty' => OK ty'
+      end.
+
+    Definition elab_type (loc: astloc) (ty: Ast.type_name) : type' :=
+      match ty with
+      | Tint8    => Tint Ctypes.I8  Ctypes.Signed
+      | Tuint8   => Tint Ctypes.I8  Ctypes.Unsigned
+      | Tint16   => Tint Ctypes.I16 Ctypes.Signed
+      | Tuint16  => Tint Ctypes.I16 Ctypes.Unsigned
+      | Tint32   => Tint Ctypes.I32 Ctypes.Signed
+      | Tuint32  => Tint Ctypes.I32 Ctypes.Unsigned
+      | Tint64   => Tlong Ctypes.Signed
+      | Tuint64  => Tlong Ctypes.Unsigned
+      | Tfloat32 => Tfloat Ctypes.F32
+      | Tfloat64 => Tfloat Ctypes.F64
+      | Tbool    => Tint Ctypes.IBool Ctypes.Signed
+      end.
+    
+    Fixpoint elab_lexp (ae: Ast.expression) : res lexp :=
+      match ae with
+      | CONSTANT c loc => OK (Econst (elab_constant loc c))
+      | VARIABLE sx loc =>
+          let x := ident_of_string sx in
+          do ty <- find_type loc x;
+          OK (Evar x ty)
+      | WHEN ae' b sx loc =>
+          let x := ident_of_string sx in
+          do ok <- assert_type loc x bool_type;
+          do e' <- elab_lexp ae';
+          OK (Ewhen e' x b)
+      | UNARY aop ae' loc =>
+          let op := elab_unop aop in
+          do e' <- elab_lexp ae';
+          do ty' <- find_type_unop loc op (typeof e');
+          OK (Eunop op e' ty')
+      | CAST aty' ae' loc =>
+          let ty' := elab_type loc aty' in
+          do e' <- elab_lexp ae';
+          OK (Eunop (CastOp ty') e' ty')
+      | BINARY aop ae1 ae2 loc =>
+          let op := elab_binop aop in
+          do e1 <- elab_lexp ae1;
+          do e2 <- elab_lexp ae2;
+          do ty' <- find_type_binop loc op (typeof e1) (typeof e2);
+          OK (Ebinop op e1 e2 ty')
+      | _ => Error (err_loc (expression_loc ae) (msg "expression not normalized"))
       end.
 
   End ElabExpressions.
 
-  Lemma has_type_In:
-    forall env x ty,
-      has_type env x ty = true ->
+  Lemma find_type_In:
+    forall env loc x ty,
+      find_type env loc x = OK ty ->
       In (x, ty) (PM.elements env).
   Proof.
-    intros env x ty Hhty.
-    unfold has_type in Hhty.
+    intros ** Hfty.
+    unfold find_type in Hfty.
     destruct (PM.find x env) eqn:Hfind; try discriminate.
-    rewrite equiv_decb_equiv in Hhty.
-    rewrite <-Hhty in Hfind.
+    injection Hfty; intro; subst.
     now apply PM.elements_correct in Hfind.
+  Qed.
+  
+  Lemma assert_type_In:
+    forall env loc x ty y,
+      assert_type env loc x ty = OK y ->
+      In (x, ty) (PM.elements env).
+  Proof.
+    intros env loc x ty y Hhty.
+    unfold assert_type in Hhty.
+    monadInv Hhty.
+    destruct (x0 ==b ty) eqn:Heq.
+    2:discriminate EQ0.
+    rewrite equiv_decb_equiv in Heq.
+    rewrite Heq in *.
+    eauto using find_type_In.
   Qed.
     
   Lemma wt_elab_clock:
-    forall env loc ast_ck ck,
-      elab_clock env loc ast_ck = OK ck ->
+    forall env loc ack ck,
+      elab_clock env loc ack = OK ck ->
       wt_clock (PM.elements env) ck.
   Proof.
-    induction ast_ck as [|ack IH]; simpl.
+    induction ack as [|ack IH]; simpl.
     now injection 1; intro; subst; auto with dftyping.
-    destruct (has_type env (ident_of_string s) bool_type) eqn:Hstr.
-    2:discriminate 1.
     intros ck Helab.
     monadInv Helab.
     constructor; auto.
-    apply has_type_In with (1:=Hstr).
+    apply assert_type_In with (1:=EQ).
   Qed.
-    
+
+  Lemma wt_elab_lexp:
+    forall env ae e,
+      elab_lexp env ae = OK e ->
+      wt_lexp (PM.elements env) e.
+  Proof.
+    induction ae; intros e Helab; monadInv Helab; constructor;
+      eauto using find_type_In, assert_type_In.
+    - unfold find_type_unop in EQ1.
+      rewrite type_unop'_correct in EQ1.
+      now DestructCases.
+    - unfold find_type_binop in EQ0.
+      match goal with H:match ?e with _ => _ end = _ |- _ =>
+        destruct e eqn:He; try discriminate; injection H end.
+      intro; subst.
+      now rewrite type_binop'_correct in He.
+    - now rewrite type_castop.
+  Qed.
 
 End ELABORATION.
+
+
+
